Fix and cleanup representation This leads to some major improvements in the ease with which I can write functions and prove things about them. Moreover, all of my proofs are much simpler now, and I have managed to get all of the theorems that I wanted to state completely stated and proved. I have removed some of the older cruft that will need to be rewritten in this new style, but at least now the file has no more sorry or oops statements in it.

isabelle/HPAPL.thy
@@ -18,160 +18,94 @@ theory HPAPL
 imports Main
 begin
 
-datatype scalar = AplInt int | AplNat nat
-datatype scalar_list = NatList "nat list" | IntList "int list"
-datatype array = Array "nat list" "scalar_list"
+class scalar =
+  fixes fill :: 'a
 
-definition Empty :: array where "Empty \<equiv> Array [0] (NatList [])"
+instantiation int and nat :: scalar
+begin
+  definition fill_int :: int where "fill_int \<equiv> 0"
+  definition fill_nat :: nat where "fill_nat \<equiv> 0"
+  instance by default
+end
 
-definition shapelst :: "array \<Rightarrow> nat list"
+datatype 'a::scalar array = Array "nat list" "'a::scalar list"
+
+definition Empty :: "'a::scalar array" where "Empty \<equiv> Array [0] []"
+
+definition shapelst :: "'a::scalar array \<Rightarrow> nat list"
 where "shapelst a \<equiv> case a of Array s v \<Rightarrow> s"
 
 definition listprod :: "nat list \<Rightarrow> nat"
 where "listprod x = foldr times x 1"
 
-fun sv2vlnat :: "nat \<Rightarrow> nat list \<Rightarrow> nat list \<Rightarrow> nat list"
-where
-    "sv2vlnat 0 orig lst = []"
-  | "sv2vlnat cnt [] lst = (replicate cnt (0::nat))"
-  | "sv2vlnat (Suc cnt) (oel # ors) [] = (oel # (sv2vlnat cnt (oel # ors) ors))"
-  | "sv2vlnat (Suc cnt) orig (elm # rst) = (elm # (sv2vlnat cnt orig rst))"
+fun sv2vl :: "nat \<Rightarrow> 'a::scalar list \<Rightarrow> 'a::scalar list \<Rightarrow> 'a::scalar list" where
+    "sv2vl 0 orig lst = []"
+  | "sv2vl cnt [] lst = (replicate cnt fill)"
+  | "sv2vl (Suc cnt) (oel # ors) [] = (oel # (sv2vl cnt (oel # ors) ors))"
+  | "sv2vl (Suc cnt) orig (elm # rst) = (elm # (sv2vl cnt orig rst))"
 
-fun sv2vlint :: "nat \<Rightarrow> int list \<Rightarrow> int list \<Rightarrow> int list"
-where
-    "sv2vlint 0 orig lst = []"
-  | "sv2vlint cnt [] lst = (replicate cnt (0::int))"
-  | "sv2vlint (Suc cnt) (oel # ors) [] = (oel # (sv2vlint cnt (oel # ors) ors))"
-  | "sv2vlint (Suc cnt) orig (elm # rst) = (elm # (sv2vlint cnt orig rst))"
+definition valuelst :: "'a::scalar array \<Rightarrow> 'a::scalar list" 
+where "valuelst a \<equiv> case a of Array s v \<Rightarrow> sv2vl (listprod s) v v"
 
-definition sv2vl :: "nat \<Rightarrow> scalar_list \<Rightarrow> scalar_list"
-where
-  "sv2vl n lst \<equiv>
-     case lst of
-       (NatList l) \<Rightarrow> NatList (sv2vlnat n l l) |
-       (IntList l) \<Rightarrow> IntList (sv2vlint n l l)"
+definition Scalar :: "'a::scalar \<Rightarrow> 'a array" 
+where "Scalar s \<equiv> Array [] [s]"
 
-definition valuelst :: "array \<Rightarrow> scalar_list" 
-where "valuelst a \<equiv> case a of Array s v \<Rightarrow> sv2vl (listprod s) v"
+definition Vector :: "'a::scalar list => 'a::scalar array" 
+where "Vector lst \<equiv> Array [length lst] lst"
 
-definition Scalar :: "scalar \<Rightarrow> array" where
-  "Scalar s \<equiv>
-     case s of
-       AplNat x \<Rightarrow> Array [] (NatList [x]) |
-       AplInt x \<Rightarrow> Array [] (IntList [x])"
-
-definition Vector :: "scalar_list => array" where 
-  "Vector lst \<equiv> 
-     case lst of
-       NatList l \<Rightarrow> Array [length l] lst |
-       IntList l \<Rightarrow> Array [length l] lst"
-
-definition natrank :: "array \<Rightarrow> nat"
+definition natrank :: "'a::scalar array \<Rightarrow> nat"
 where "natrank a \<equiv> length (shapelst a)"
 
 lemma natrank_Empty [simp]: "natrank Empty = 1"
 by (simp add: Empty_def natrank_def shapelst_def)
 
 lemma natrank_Scalar [simp]: "natrank (Scalar x) = 0"
-by (simp add: natrank_def Scalar_def shapelst_def) (split scalar.split, simp)
+by (simp add: natrank_def Scalar_def shapelst_def)
 
-definition vec2lst :: "array \<Rightarrow> scalar_list"
+definition vec2lst :: "'a::scalar array \<Rightarrow> 'a::scalar list"
 where "vec2lst vec \<equiv> case vec of Array s v \<Rightarrow> v"
 
-theorem vector_shape [simp]: "shapelst (Vector (NatList s)) = [length s]"
-by (simp add: Vector_def shapelst_def)
-
-theorem vector_shape2 [simp]: "shapelst (Vector (IntList s)) = [length s]"
+theorem vector_shape [simp]: "shapelst (Vector s) = [length s]"
 by (simp add: Vector_def shapelst_def)
 
 theorem vector_rank [simp]: "natrank (Vector s) = 1"
-by (simp add: Vector_def natrank_def shapelst_def) 
-   (split scalar_list.split, simp)
+by (simp add: Vector_def natrank_def shapelst_def)
 
 theorem vector_inverse [simp]: "vec2lst (Vector lst) = lst"
-by (simp add: Vector_def vec2lst_def, split scalar_list.split, simp)
+by (simp add: Vector_def vec2lst_def)
 
-theorem vector_empty: "Vector (NatList []) = Empty"
+theorem vector_empty: "Vector [] = Empty"
 by (simp add: Vector_def Empty_def)
 
-theorem vec2lst_empty [simp]: "vec2lst Empty = (NatList [])"
+theorem vec2lst_empty [simp]: "vec2lst Empty = []"
 by (simp add: Empty_def vec2lst_def)
 
-definition shape :: "array \<Rightarrow> array" 
-where "shape a \<equiv> Vector (NatList (shapelst a))"
+definition shape :: "'a::scalar array \<Rightarrow> nat array" 
+where "shape a \<equiv> Vector (shapelst a)"
 
-theorem shape_Empty [simp]: "shape Empty = Vector (NatList [0])"
+theorem shape_Empty [simp]: "shape Empty = Vector [0]"
 by (simp add: shape_def Empty_def shapelst_def)
 
 theorem rank_shape_one [simp]: "natrank (shape a) = 1" 
 by (auto simp: shape_def)
 
-theorem shape2_rank [simp]: "shape (shape a) = Vector (NatList [natrank a])"
+theorem shape2_rank [simp]: "shape (shape a) = Vector [natrank a]"
 by (auto simp: shape_def natrank_def)
 
-theorem shape3_is_one [simp]: "shape (shape (shape a)) = Vector (NatList [1])"
+theorem shape3_is_one [simp]: "shape (shape (shape a)) = Vector [1]"
 by (auto simp: shape_def)
 
 theorem shape_scalar [simp]: "shape (Scalar x) = Empty"
 by (simp add: shape_def Empty_def Vector_def Scalar_def shapelst_def)
-   (split scalar.split, simp)
-
-definition slget :: "scalar_list \<Rightarrow> nat \<Rightarrow> scalar" where
-  "slget l i \<equiv>
-     case l of
-         NatList v \<Rightarrow> AplNat (v ! i)
-       | IntList v \<Rightarrow> AplInt (v ! i)"
 
 definition index_unraveled :: "nat list \<Rightarrow> nat list \<Rightarrow> nat"
 where "index_unraveled s i \<equiv> 0"
 
-definition indexer :: "nat list \<Rightarrow> nat list \<Rightarrow> scalar_list \<rightharpoonup> scalar" where
-  "indexer i s d \<equiv> 
-     if (list_all2 op < i s)
-     then Some (slget d (index_unraveled s i))
-     else None"
+definition index :: "nat array \<Rightarrow> 'a::scalar array \<Rightarrow> 'a" where
+"index i a \<equiv> (valuelst a) ! index_unraveled (shapelst a) (valuelst i)"
 
-definition indexerint :: "int list \<Rightarrow> nat list \<Rightarrow> scalar_list \<rightharpoonup> scalar" where
-  "indexerint i s d \<equiv> 
-     if (list_all2 op > i (replicate (length i) 0))
-     then indexer (map nat i) s d
-     else None"
-
-definition index :: "array \<Rightarrow> array \<rightharpoonup> scalar" where 
-  "index i a \<equiv> 
-     case (i, a) of
-         (Array [n] (NatList v), (Array s d)) \<Rightarrow> indexer v s d
-       | (Array [n] (IntList v), (Array s d)) \<Rightarrow> indexerint v s d
-       | other \<Rightarrow> None"
-
-theorem index_scalar [simp]: "index Empty (Scalar x) = Some x"
-by sorry
-
-definition releach :: "(scalar \<Rightarrow> scalar \<Rightarrow> bool) \<Rightarrow> array \<Rightarrow> array \<Rightarrow> bool"
-where "releach f a b \<equiv> 
-  (shapelst a = (shapelst b) \<and> (list_all2 f (valuelst a) (valuelst b)))
-   \<or> (natrank a = 0 
-      \<and> (list_all2 f 
-          (sv2vl (listprod (shapelst b)) (valuelst a)) 
-          (valuelst b)))
-   \<or> (natrank b = 0 
-      \<and> (list_all2 f 
-          (valuelst a) 
-          (sv2vl (listprod (shapelst a)) (valuelst b))))"
-
-definition monmap :: "('a \<Rightarrow> 'b) \<Rightarrow> (nat list \<rightharpoonup> 'a) \<Rightarrow> (nat list \<rightharpoonup> 'b)"
-where "monmap fn v i \<equiv> Option.map fn (v i)"
-
-lemma monmap_dom [simp]: "dom (monmap fn v) = dom v"
-by (auto simp: monmap_def dom_option_map)
-
-definition monseach :: "('a \<Rightarrow> 'b) \<Rightarrow> 'a array \<Rightarrow> 'b array"
-where "monseach fn a \<equiv> Array (shapelst a) (monmap fn (arrvmap a))"
-
-theorem monseach_shape [simp]: "shapelst (monseach fn a) = shapelst a"
-by sorry
-
-theorem monseach_rank [simp]: "rank (monseach fn a) = rank a"
-by sorry
+theorem index_scalar [simp]: "index Empty (Scalar x) = x"
+by (simp add: Scalar_def Empty_def index_def index_unraveled_def 
+              valuelst_def listprod_def)
 
 end
